Xlone-Main.dfy
@@ -1,0 +1,1186 @@
+include "Xlone.dfy"
+include "Xlone-Seed.dfy"
+include "Graphing.dfy"
+
+const protoTypesX : map<string, Mode> :=
+      map["jat":= Evil]
+         ["dat":= Evil]
+         ["cat":= Evil]
+         ["rat":= Evil]
+         ["nxt":= Evil]
+         ["eye":= Evil]
+         ["kye":= Evil]
+         ["lat":= Evil]
+         ["fucker" := Evil]
+
+
+method {:verify false} XloneMain(s : seq<string>)
+ decreases *
+{
+  print "Main()\n";
+
+ if ((|s| > 1) && (|s[1]| > 0)) {
+
+  print "xxx", (s[1][0]), "xxx\n";
+
+   match (s[1][0]) {
+     case '0' =>  Main0();
+     case '1' =>  Main1(s[2..]);
+     case '2' =>  Main2();
+     case '3' =>  Main3();
+     case '4' =>  Main4();
+     case _ => {}
+  }
+  print "Exit, pursued by a bear\n";
+ }
+}
+
+
+//{:verify false} //{:only}
+method makeDemo() returns (t : Object, a : Object, b : Object, os : set<Object>)
+  ensures t in os
+  ensures a in os
+  ensures b in os
+  ensures forall o <- os :: o.Ready()
+//  ensures forall o <- os :: o.AllOwnersAreWithinThisHeap(os)
+  ensures forall o <- os :: o.AllOutgoingReferencesWithinThisHeap(os)
+  ensures forall o <- os :: o.fieldModes == protoTypesX
+  ensures COK(a, os)
+  ensures CallOK(os)
+  ensures {"eye","kye"} <=  a.fields.Keys
+  ensures {"lat", "dat", "cat", "rat"} <= a.fields["eye"].fields.Keys
+{
+
+assert CallOK({}, {}) by { NothingShallComeOfNothing({}, {}); }
+
+t := new Object.make(protoTypesX, {}, {}, "t");
+//   t
+//   a      b c
+//   d        cc
+//   e f g h
+
+assert t.Ready();
+assert COK(t, {t}) by { reveal COK(); }
+
+// protoTypesX 8-)
+// cat dat eye fucker jat kye lat nxt rat/
+
+assert t.AMFX == {};
+assert forall o : Object <- {t}, ooo <- o.AMFO :: o.AMFO >= ooo.AMFO;
+
+assert CallOK({t},{t}) by { reveal COK(), CallOK(); }
+
+a := new Object.make(protoTypesX, {t}, {t}, "a");
+
+b := new Object.make(protoTypesX, {t}, {t}, "b");
+
+var c := new Object.make(protoTypesX, {t}, {t}, "c");
+
+reveal CallOK(), COK();
+assert CallOK({c}, {t,c});
+var cc := new Object.make(protoTypesX, {c}, {t,c}, "cc");
+
+
+reveal CallOK(), COK();
+assert CallOK({a}, {t,a});
+var d := new Object.make(protoTypesX, {a}, {t,a}, "d");
+
+assert CallOK({d}, {t,a,d});
+var e := new Object.make(protoTypesX, {d}, {t,a,d}, "e"); //we're gonna clone this one..?
+
+assert CallOK({e}, {t,a,d,e});
+var f := new Object.make(protoTypesX, {e}, {t,a,d,e}, "f");
+
+assert CallOK({f},  {t,a,d,e,f});
+var g := new Object.make(protoTypesX, {f},  {t,a,d,e,f},   "g");
+
+assert CallOK({g}, {t,a,d,e,f,g});
+var h := new Object.make(protoTypesX, {g}, {t,a,d,e,f,g}, "h");
+
+assert CallOK({g}, {t,a,d,e,f,g});
+var i := new Object.make(protoTypesX, {g}, {t,a,d,e,f,g}, "i");
+assert CallOK({e}, {t,a,d,e,f,g,h});
+var j := new Object.make(protoTypesX, {e}, {t,a,d,e,f,g,h}, "j");
+assert CallOK({e}, {t,a,d,e,f,g,h});
+var k := new Object.make(protoTypesX, {e}, {t,a,d,e,f,g,h}, "k");
+assert CallOK({e},  {t,a,d,e,f,g,h});
+var l := new Object.make(protoTypesX, {e}, {t,a,d,e,f,g,h}, "l");
+
+
+assert t.Ready();
+
+assert a.Ready();
+assert b.Ready();
+assert c.Ready();
+assert d.Ready();
+assert e.Ready();
+assert f.Ready();
+assert g.Ready();
+assert h.Ready();
+assert i.Ready();
+assert j.Ready();
+assert k.Ready();
+assert l.Ready();
+
+os := {t,   a, b, c, cc, d, e, f, g, h, i, j, k, l};
+var ot := [t,   a, b, c, cc, d, e, f, g, h, i, j, k, l];
+
+a.fields := map["eye":=d]["kye":=c];
+c.fields := map["eye":=cc];
+d.fields := map["lat":= e]["dat":=f]["cat":=g]["rat":= h];
+e.fields := map["eye":=f];
+f.fields := map["nxt":=l];
+l.fields := map["nxt":=j];
+j.fields := map["nxt":=k];
+
+assert COK(a,os);
+
+assert d.AllFieldsAreDeclared();
+assert d.AllFieldsContentsConsistentWithTheirDeclaration();
+assert d.AllOutgoingReferencesAreOwnership(os);
+
+print "REALLY REALLY DAVE? ", d.AllOutgoingReferencesAreOwnership(os),"\n";
+print "why am I printing out all the fields of object d? - \n";
+printobjfields(d);
+
+
+assert d.AllOutgoingReferencesAreOwnership(os);
+
+assert d.AllOutgoingReferencesWithinThisHeap(os);
+assert COK(d,os);
+
+assert CallOK(os);
+
+}
+
+// {:verify false} //{:only}
+method {:verify false} Main0()
+  decreases *
+{
+
+print "Main0\n";
+
+var t, a, b, os := makeDemo();
+var orig := os;
+var oq := set2seq(os);
+
+assert forall o : Object <- os :: (o.Ready());
+
+print "|os| == ", |os|, "\n";
+
+print "+++++++++++++\n";
+print "original store (os)\n";
+print "+++++++++++++\n";
+printobjectset(os);
+print "+++++++++++++\n";
+
+print "done setup\n";
+
+//assert isIsomorphicMappingOWNED(d, d, isomap, os);
+
+// var ros := walkies(d, d, isomap, os);
+
+print "%%%%%%%%%%%%%%%%%%%%%%%%%%%%%%%%%%%%%%%%%%%%%%%%%%%%%%%%%%%%%%\n";
+
+print "about to Xlone a\n";
+
+assert CallOK(os);
+assert COK(a, os);
+assert CallOK(a.owner,os) by { reveal COK(), CallOK(); }
+
+assert forall o <- os :: (o.Ready());
+//assert forall o <- os :: (o.AllOwnersAreWithinThisHeap(os));
+
+assert forall x <- os ::  x.AllOutgoingReferencesWithinThisHeap(os);
+
+
+////////////////////////////////////////////////////////////
+
+var k := a;
+
+var m : Klon := seed(k, {b}, os);
+
+
+//
+//
+//
+//
+// /// PREGRAPH
+// /// PREGRAPH
+// /// PREGRAPH
+// /// PREGRAPH
+// /// PREGRAPH
+//
+//
+//       print "\n\n//STARTGRAPH\n";
+//       print "////////////////////////////////////////////////////////////////////////////////\n";
+//       print "////////////////////////////////////////////////////////////////////////////////\n";
+//       print "////////////////////////////////////////////////////////////////////////////////\n";
+//       print "//  ", "CLONEY=WONEY", "\n";
+//
+// //  gops := GraphOptions(graph, lines, nodes, extra);
+// var gops := GraphOptions("",    "OF",  "",    "");
+//
+//   print "\n\ndigraph dafny {\n";
+//   print "   rankdir=\"BT\";\n";
+//   print "   layers=\"mapping:fields:owner:bound:amfo:bg\";\n";
+//   print "   node [shape=box]\n\n";
+//
+//   graphobjectset(os, m, gops);
+//
+//   graphmapping(m.m, gops);
+//
+//  //   graphrefs(os, gops);
+//
+//  print "}\n\n\n";
+//
+//     print "//ENDGRAPH\n";
+//     print "////////////////////////////////////////////////////////////////////////////////\n";
+//     print "///////////////////////////////////////////////////////////////////////////////\n";
+//     print "////////////////////////////////////////////////////////////////////////////////\n";
+//
+//
+// /// PREGRAPH
+// /// PREGRAPH
+// /// PREGRAPH
+// /// PREGRAPH
+// /// PREGRAPH
+//
+//
+
+
+
+
+
+
+
+
+
+
+
+
+
+
+//at this point we've got all the owners in the map
+//what we DON"T have is the object itself. So:
+
+
+
+var v := new Object.make(k.fieldModes, m.clowner, m.oHeap, "clone_of_" + k.nick, m.clbound);
+
+m := m.CalidKV(k,v);
+
+var rm := Xlone_All_Fields(k,v,m);
+var ra := v;
+m := rm;
+
+os := m.hns();
+
+/// POSTGRAPH
+/// POSTGRAPH
+/// POSTGRAPH
+/// POSTGRAPH
+/// POSTGRAPH
+
+
+      print "\n\n//STARTGRAPH\n";
+      print "////////////////////////////////////////////////////////////////////////////////\n";
+      print "////////////////////////////////////////////////////////////////////////////////\n";
+      print "////////////////////////////////////////////////////////////////////////////////\n";
+      print "//  ", "CLONEY=WONEY", "\n";
+
+//  gops := GraphOptions(graph, lines, nodes, extra);
+var gops := GraphOptions("",    "OF",  "",    "");
+
+  print "\n\ndigraph dafny {\n";
+  print "   rankdir=\"BT\";\n";
+  print "   layers=\"mapping:fields:owner:bound:amfo:bg\";\n";
+  print "   node [shape=box]\n\n";
+
+  graphobjectset(os, m, gops);
+
+  graphmapping(m.m, gops);
+
+ //   graphrefs(os, gops);
+
+ print "}\n\n\n";
+
+    print "//ENDGRAPH\n";
+    print "////////////////////////////////////////////////////////////////////////////////\n";
+    print "///////////////////////////////////////////////////////////////////////////////\n";
+    print "////////////////////////////////////////////////////////////////////////////////\n";
+
+
+/// POSTGRAPH
+/// POSTGRAPH
+/// POSTGRAPH
+/// POSTGRAPH
+/// POSTGRAPH
+
+
+
+
+
+
+
+
+
+assert a in rm.m.Keys;
+assert rm.from(m);
+assert m.Calid();
+assert m.ownersInKlown(a);
+
+print "+++++++++++++\n";
+print "original store (orig)\n";
+print "+++++++++++++\n";
+printobjectset(orig);
+print "+++++++++++++\n";
+print "clones rm.Values - orig\n";
+print "+++++++++++++\n";
+printobjectset(rm.m.Values - orig);
+print "+++++++++++++\n";
+printmapping(rm.m);
+//
+// print "\n\n\n\nwaiting...\\n\n";
+//
+// var context : set<Object> := rm.oHeap + rm.ns();
+// assert os <= context;
+// assert rm.m.Values <= context;
+//
+// var oz := set2seq(context);
+//
+//
+//
+// // var result : bool :=  jeSuisClone(a, rm, context);
+//
+// var result : bool :=  istEinKlon(c, rm, context);
+//
+// print "istEinKlon = ", result;
+//
+// print "\n\n";
+//
+// print "\n$$$$$$$$$$$$$$$$$$\n";
+// //                HeyHoLetsGo(rm);
+//
+//
+//       for i := 0 to |oz|
+//        {
+//          printobj(oz[i]);
+//          print "  AMFO==";
+//          printown(oz[i].AMFO);
+//
+//         var oo := oz[i].AMFO;
+//         if (oo >= rm.o.AMFO) { print "  (inside)\n"; } else { print "  (outside)\n";}
+//
+//         if (oz[i] in rm.m.Keys)  {
+//             print "  mapsto ";
+//             printobj(rm.m[oz[i]]);
+//
+//             if (oz[i].AMFO <= rm.m.Keys)
+//               {
+//                 print "\n mapThruKlon ==";
+//                 printown( mapThruKlon(oo, rm));
+//                 print "\n   calc      ==";
+//                 // printown( calculateClownership(oo, rm));
+//                 // print "\n   mTKlown   ==";
+//                 // printown( mapThruKlown(oo, rm));
+//                 // print "\n   mTKlownII ==";
+//                 // printown( mapThruKlownIfInside(oo, rm));
+//                 // print "\n   OLDmapTKl ==";
+//                 // printown( OLDmapThruKlown(oo, rm));
+//               }
+//              else
+//              {
+//               print "  but AMFO not in Keys??? extra bits:";
+//               printown( oz[i].AMFO - rm.m.Keys );
+//              }
+//             print "\n";
+//         }
+//         else {
+//           print "  NOT IN rm.m\n";
+//         }
+//
+//        }
+//
+//
+
+print "\n$$$$$$$$$$$$$$$$$$\n";
+
+
+print "\nDone\n";
+}
+// end
+
+
+method {:verify false} Main1(s : seq<string>)
+ decreases *
+ {
+
+
+print "Main1\n";
+
+for x := 0 to |s| {
+  print x, "  ", s[x],"\n";
+}
+
+var t := new Object.make(protoTypesX, {}, {}, "kernel");
+var a := new Object.make(protoTypesX, {t}, {t},         "screen");
+var b := new Object.make(protoTypesX, {a}, {t},         "window1");
+var c := new Object.make(protoTypesX, {b}, {t},         "textbox");
+var d := new Object.make(protoTypesX, {a}, {a,t},       "font");
+var e := new Object.make(protoTypesX, {a}, {a,t},       "window2");
+var f := new Object.make(protoTypesX, {b}, {t,a,c},     "text");
+var g := new Object.make(protoTypesX, {f}, {t,a,c,f},   "line1");
+var h := new Object.make(protoTypesX, {f}, {t,a,c,f,g}, "line2");
+var i := new Object.make(protoTypesX, {f}, {t,a,d},     "line3");
+// var j := new Object.make(protoTypesX, {c}, {t,a,d},     "j");
+// var k := new Object.make(protoTypesX, {c}, {t,a,e},     "k");
+// var l := new Object.make(protoTypesX, {c}, {t,a,e},     "l");
+
+a.fields := map["font":=d,"win":=b];
+b.fields := map["next":=e,"sub":=c];
+c.fields := map["font":=d,"text":=f];
+f.fields := map["nxt":=g,"1":=g,"2":=h,"3":=i,"fnt":=d];
+g.fields := map["nxt":=h];
+h.fields := map["nxt":=i];
+
+
+
+var os : set<Object> := {t,   a, b, c, d, e, f, g, h, i };//, j, k, l };
+var oq : seq<Object> := [t,   a, b, c, d, e, f, g, h, i ];//, j, k, l ];
+
+print "|os| == ", |os|, "\n";
+var orig := os;
+
+// print "+++++++++++++\n";
+// print "original store (os)\n";
+// print "+++++++++++++\n";
+// printobjectset(os);
+// print "+++++++++++++\n";
+
+print "done setup\n";
+
+//assert isIsomorphicMappingOWNED(d, d, isomap, os);
+
+// var ros := walkies(d, d, isomap, os);
+
+print "%%%%%%%%%%%%%%%%%%%%%%%%%%%%%%%%%%%%%%%%%%%%%%%%%%%%%%%%%%%%%%\n";
+
+print "about to Xlone a\n";
+
+assert CallOK(os);
+assert COK(a, os);
+assert CallOK(a.owner,os) by { reveal COK(), CallOK(); }
+
+assert forall o <- os :: (o.Ready());
+//assert forall o <- os :: (o.AllOwnersAreWithinThisHeap(os));
+
+assert forall x <- os ::  x.AllOutgoingReferencesWithinThisHeap(os);
+
+/////////////////////////////////////////////////////       ///////
+
+var m : Klon := seed(t,{t},os);
+
+if ((|s| > 0) && (|s[0]| > 0)) {
+    if (s[0][0] == 'd')  // deeep
+        {
+          var k := a;
+      m := seed(k, {t}, os);
+      var v := new Object.make(k.fieldModes, m.clowner, m.oHeap, "clone_of_" + k.nick, m.clbound);
+      m := m.CalidKV(k,v);
+      var rm := Xlone_All_Fields(k,v,m);
+      var ra := v;
+      m := rm;
+        }
+      else if (s[0][0] == 's')  // shallow
+      {
+        var k := f;
+      m := seed(k, {b}, os);
+      var v := new Object.make(k.fieldModes, m.clowner, m.oHeap, "clone_of_" + k.nick, m.clbound);
+      m := m.CalidKV(k,v);
+      v.fields :=   k.fields;
+      var rm := m;
+      var ra := v;
+      m := rm;
+      }
+ }
+
+
+
+
+
+
+os := m.hns();
+
+/// POSTGRAPH
+/// POSTGRAPH
+/// POSTGRAPH
+/// POSTGRAPH
+/// POSTGRAPH
+
+
+      print "\n\n//STARTGRAPH\n";
+      print "////////////////////////////////////////////////////////////////////////////////\n";
+      print "////////////////////////////////////////////////////////////////////////////////\n";
+      print "////////////////////////////////////////////////////////////////////////////////\n";
+      print "//  ", "CLONEY=WONEY", "\n";
+
+//  gops := GraphOptions(graph, lines, nodes, extra);
+var gops := GraphOptions("",    "OF",  "",    "");
+
+  print "\n\ndigraph dafny {\n";
+  print "   rankdir=\"TB\";\n";
+  print "   layers=\"mapping:fields:owner:bound:amfo:bg\";\n";
+  print "   node [shape=box]\n\n";
+
+  print "{rank=same}\n";
+
+  //pencolor=invis;
+
+  print "subgraph cluster1 {pencolor=invis; kernel; subgraph cluster11 {pencolor=invis; screen; window1; textbox; window2 font} }\n";
+  print "subgraph cluster2 {pencolor=invis; text; line1; line2; line3;}\n";
+
+  graphobjectset(os, m, gops);
+
+  graphmapping(m.m, gops);
+
+ //   graphrefs(os, gops);
+
+ print "}\n\n\n";
+
+    print "//ENDGRAPH\n";
+    print "////////////////////////////////////////////////////////////////////////////////\n";
+    print "///////////////////////////////////////////////////////////////////////////////\n";
+    print "////////////////////////////////////////////////////////////////////////////////\n";
+
+
+/// POSTGRAPH
+/// POSTGRAPH
+/// POSTGRAPH
+/// POSTGRAPH
+/// POSTGRAPH
+
+
+
+
+
+//
+//
+//
+//
+// assert a in rm.m.Keys;
+// assert rm.from(m);
+// assert m.Calid();
+// assert m.ownersInKlown(a);
+//
+// print "+++++++++++++\n";
+// print "original store (orig)\n";
+// print "+++++++++++++\n";
+// printobjectset(orig);
+// print "+++++++++++++\n";
+// print "clones rm.Values - orig\n";
+// print "+++++++++++++\n";
+// printobjectset(rm.m.Values - orig);
+// print "+++++++++++++\n";
+// printmapping(rm.m);
+
+
+
+// print "\n\n\n\nwaiting...\\n\n";
+//
+// var context : set<Object> := rm.oHeap + rm.ns();
+// assert os <= context;
+// assert rm.m.Values <= context;
+//
+// var oz := set2seq(context);
+//
+//
+//
+// // var result : bool :=  jeSuisClone(a, rm, context);
+//
+// var result : bool :=  istEinKlon(c, rm, context);
+//
+// print "istEinKlon = ", result;
+//
+// print "\n\n";
+//
+// print "\n$$$$$$$$$$$$$$$$$$\n";
+// //                HeyHoLetsGo(rm);
+//
+//
+//       for i := 0 to |oz|
+//        {
+//          printobj(oz[i]);
+//          print "  AMFO==";
+//          printown(oz[i].AMFO);
+//
+//         var oo := oz[i].AMFO;
+//         if (oo >= rm.o.AMFO) { print "  (inside)\n"; } else { print "  (outside)\n";}
+//
+//         if (oz[i] in rm.m.Keys)  {
+//             print "  mapsto ";
+//             printobj(rm.m[oz[i]]);
+//
+//             if (oz[i].AMFO <= rm.m.Keys)
+//               {
+//                 print "\n mapThruKlon ==";
+//                 printown( mapThruKlon(oo, rm));
+//                 print "\n   calc      ==";
+//                 // printown( calculateClownership(oo, rm));
+//                 // print "\n   mTKlown   ==";
+//                 // printown( mapThruKlown(oo, rm));
+//                 // print "\n   mTKlownII ==";
+//                 // printown( mapThruKlownIfInside(oo, rm));
+//                 // print "\n   OLDmapTKl ==";
+//                 // printown( OLDmapThruKlown(oo, rm));
+//               }
+//              else
+//              {
+//               print "  but AMFO not in Keys??? extra bits:";
+//               printown( oz[i].AMFO - rm.m.Keys );
+//              }
+//             print "\n";
+//         }
+//         else {
+//           print "  NOT IN rm.m\n";
+//         }
+//
+//        }
+//
+//
+
+print "\n$$$$$$$$$$$$$$$$$$\n";
+
+
+print "\nDone\n";
+
+}
+// end
+
+
+
+
+
+
+
+
+method {:verify false} Main2() {
+
+print "main showing RefOK etc\n";
+
+var t := new Object.make(protoTypesX, {}, {}, "t");
+
+//   t
+//   a       b       c
+//   d  e            f
+//  ij kl            g
+//                   h
+
+var a := new Object.make(protoTypesX, {t}, {t},         "a");
+var b := new Object.make(protoTypesX, {t}, {t},         "b");
+var c := new Object.make(protoTypesX, {t}, {t},         "c");
+var d := new Object.make(protoTypesX, {a}, {a,t},       "d");
+var e := new Object.make(protoTypesX, {a}, {a,t},       "e");
+var f := new Object.make(protoTypesX, {c}, {t,a,c},     "f");
+var g := new Object.make(protoTypesX, {f}, {t,a,c,f},   "g");
+var h := new Object.make(protoTypesX, {g}, {t,a,c,f,g}, "h");
+var i := new Object.make(protoTypesX, {c}, {t,a,d},     "i");
+var j := new Object.make(protoTypesX, {c}, {t,a,d},     "j");
+var k := new Object.make(protoTypesX, {c}, {t,a,e},     "k");
+var l := new Object.make(protoTypesX, {c}, {t,a,e},     "l");
+
+
+var os : set<Object> := {t,   a, b, c, d, e, f, g, h, i, j, k, l };
+var oq : seq<Object> := [t,   a, b, c, d, e, f, g, h, i, j, k, l ];
+
+assert forall o <- oq :: o.Ready();
+
+//   for i := 0 to |oq|
+//     {
+//       var o : Object := oq[i];
+//
+//       assert o.Ready();
+//
+//       print "\n=============================================================\n";
+//       print "=============================================================\n";
+//
+//       printobject(o);
+//     }
+//    print "\n\n";
+
+
+print "\n\nOwnership - Inside =========================\n";
+print "Ownership - Inside =========================\n\n";
+
+//       for i := 0 to |oq|
+//        {
+//          printobj(oq[i]);
+//          print "  ";
+//
+//          for j := 0 to |oq|
+// {
+//          print (if (inside(oq[i],oq[j])) then "i" else " ");
+//          print " ";
+// }
+//          print "\n";
+//
+//        }
+//   print "\n\n";
+
+      for i := 0 to |oq|
+       {
+        print oq[i].nick;
+//         printobj(oq[i]);
+         print "  ";
+
+         for j := 0 to |oq|
+{
+         print (if (inside(oq[i],oq[j])) then (oq[i].nick+"<="+oq[j].nick) else "    ");
+         print " ";
+}
+         print "\n";
+
+       }
+  print "\n\n";
+  print "\n[\n";
+
+      for i := 0 to |oq|
+       {
+         print "\"";
+
+         for j := 0 to |oq|
+{
+         print (if (inside(oq[i],oq[j])) then ("x") else " ");
+}
+         if (i < (|oq|-1))  { print "\",\n";} else { print "\"\n";}
+
+       }
+print "]\n";
+
+
+
+
+
+var matrix : seq<string>:= [
+"x            ",
+"xx           ",
+"x x          ",
+"x  x         ",
+"xx  x        ",
+"xx   x       ",
+"x  x  x      ",
+"x  x  xx     ",
+"x  x  xxx    ",
+"x  x     x   ",
+"x  x      x  ",
+"x  x       x ",
+"x  x        x"
+];
+
+  print "\n\n";
+
+      for i := 0 to |matrix|
+       {
+         for j := 0 to |matrix[0]|
+          {
+         print match (inside(oq[i],oq[j]), (matrix[i][j]) )
+           case (true,  'x') => "o"  //OK, true positive
+           case (true,  ' ') => "F"  //false positive
+           case (false, ' ') => " "  //OK, true negative
+           case (false, 'x') => "M"; //false negative
+          }
+         print "\n";
+       }
+print "\n";
+
+
+
+print "ownerInsideOwner ownerInsideOwner ownerInsideOwner ownerInsideOwner\n";
+print "ownerInsideOwner ownerInsideOwner ownerInsideOwner ownerInsideOwner\n";
+
+      for i := 0 to |matrix|
+       {
+         for j := 0 to |matrix[0]|
+          {
+         print match (ownerInsideOwner(oq[i].AMFO,oq[j].AMFO), (matrix[i][j]) )
+           case (true,  'x') => "o"  //OK
+           case (true,  ' ') => "M"  //missing
+           case (false, ' ') => " "
+           case (false, 'x') => "F"; //false posiutive, ie FUCKED
+          }
+         print "\n";
+       }
+print "\n";
+
+
+print "FUCKED FUCKED FUCKED FUCKED FUCKED\n";
+print "FUCKED FUCKED FUCKED FUCKED FUCKED\n";
+
+print "\n\nREFERENCE OK refOK =========================\n";
+print "REFERENCE OK refOK =========================\n\n";
+
+      for i := 0 to |oq|
+       {
+         print oq[i].nick;
+         //printobj(oq[i]);
+         print "  ";
+
+         for j := 0 to |oq|
+{
+         print (if (refOK(oq[i],oq[j])) then (oq[i].nick+"->"+oq[j].nick) else "    ");
+         print " ";
+}
+print "\n";
+}
+
+//uncomment to print out a new "matrix"
+//
+//
+//   print "\n[\n";
+//
+//       for i := 0 to |oq|
+//        {
+//          print "\"";
+//
+//          for j := 0 to |oq|
+// {
+//          print (if (refOK(oq[i],oq[j])) then ("x") else " ");
+// }
+//          if (i < (|oq|-1))  { print "\",\n";} else { print "\"\n";}
+//
+//        }
+// print "]\n";
+
+
+var keanu :=
+[
+"xxxx         ",
+"xxxxxx       ",
+"xxxx         ",
+"xxxx  x  xxxx",
+"xxxxxx       ",
+"xxxxxx       ",
+"xxxx  xx xxxx",
+"xxxx  xxxxxxx",
+"xxxx  xxxxxxx",
+"xxxx  x  xxxx",
+"xxxx  x  xxxx",
+"xxxx  x  xxxx",
+"xxxx  x  xxxx"
+];
+
+
+  print "\n\n";
+
+      for i := 0 to |keanu|
+       {
+         for j := 0 to |keanu[0]|
+          {
+         print match (refOK(oq[i],oq[j]), (keanu[i][j]) )
+           case (true,  'x') => "o"  //OK, true positive
+           case (true,  ' ') => "F"  //false positive
+           case (false, ' ') => " "  //OK, true negative
+           case (false, 'x') => "M"; //false negative
+          }
+         print "\n";
+       }
+print "\n";
+
+
+print "\nDone\n\n";
+
+
+
+
+
+}
+
+// end main2
+
+
+
+
+method {:verify false} Main3() {
+
+print "main poking at bound etc\n";
+print "Object G has bound at object t\n";
+
+var t := new Object.make(protoTypesX, {}, {}, "t");
+
+//   t
+//   a       b       c
+//   d  e            f
+//  ij kl            g
+//                   h
+
+var a := new Object.make(protoTypesX, {t}, {t},         "a");
+var b := new Object.make(protoTypesX, {t}, {t},         "b");
+var c := new Object.make(protoTypesX, {t}, {t},         "c");
+var d := new Object.make(protoTypesX, {a}, {a,t},       "d");
+var e := new Object.make(protoTypesX, {a}, {a,t},       "e");
+var f := new Object.make(protoTypesX, {c}, {t,a,c},     "f");
+var g := new Object.make(protoTypesX, {f}, {t,a,c,f},   "G", {t});
+var h := new Object.make(protoTypesX, {g}, {t,a,c,f,g}, "H", {g});
+var i := new Object.make(protoTypesX, {d}, {t,a,d},     "i");
+var j := new Object.make(protoTypesX, {d}, {t,a,d},     "j");
+var k := new Object.make(protoTypesX, {e}, {t,a,e},     "k");
+var l := new Object.make(protoTypesX, {e}, {t,a,e},     "l");
+
+print "a->d : ", refOK(a,d), "\n";
+print "a->e : ", refOK(a,e), "\n";
+
+var os : set<Object> := {t,   a, b, c, d, e, f, g, h, i, j, k, l };
+var oq : seq<Object> := [t,   a, b, c, d, e, f, g, h, i, j, k, l ];
+
+assert forall o <- oq :: o.Ready();
+
+print "\n\nREFERENCE OK refOK =========================\n";
+print "REFERENCE OK refOK =========================\n\n";
+
+      for i := 0 to |oq|
+       {
+         print oq[i].nick;
+         //printobj(oq[i]);
+         print "  ";
+
+         for j := 0 to |oq|
+{
+         print (if (refOK(oq[i],oq[j])) then (oq[i].nick+"->"+oq[j].nick) else "    ");
+         print " ";
+}
+print "\n";
+}
+
+
+
+
+  print "\n[\n";
+
+      for i := 0 to |oq|
+       {
+         print "\"";
+
+         for j := 0 to |oq|
+{
+         print (if (refOK(oq[i],oq[j])) then ("x") else " ");
+}
+         if (i < (|oq|-1))  { print "\",\n";} else { print "\"\n";}
+
+       }
+print "]\n";
+
+
+var keanu :=
+[
+"xxxx         ",
+"xxxxxx       ",
+"xxxx         ",
+"xxxx  x  xxxx",
+"xxxxxx       ",
+"xxxxxx       ",
+"xxxx  xx xxxx",
+"xxxx  xxxxxxx",
+"xxxx  xxxxxxx",
+"xxxx  x  xxxx",
+"xxxx  x  xxxx",
+"xxxx  x  xxxx",
+"xxxx  x  xxxx"
+];
+
+
+  print "\n\n";
+
+      for i := 0 to |keanu|
+       {
+         for j := 0 to |keanu[0]|
+          {
+         print match (refOK(oq[i],oq[j]), (keanu[i][j]) )
+           case (true,  'x') => "o"  //OK, true positive
+           case (true,  ' ') => "F"  //false positive
+           case (false, ' ') => " "  //OK, true negative
+           case (false, 'x') => "M"; //false negative
+          }
+         print "\n";
+       }
+print "\n";
+
+
+print "\nDone\n\n";
+
+
+
+
+
+} //end Main3
+
+
+method {:verify false} Main4() {
+
+print "long and thin study of bounds\n";
+
+var t := new Object.make(protoTypesX, {}, {}, "t");  //top;
+
+print "   t\n";
+
+var depth  : nat := 5;
+var prev   := t;
+var os := {t};
+var oq := [t];
+
+var o2 : Object? := null;
+
+for i := 0 to depth
+{
+  var spine := new Object.make(protoTypesX, {prev}, os, "o"+natToString(i));
+
+  if (i == 1)  {o2 := prev;}
+
+  var pbound := {prev};
+  if (i == 2) {pbound := {};}
+  if (i == 3) {pbound := {o2};}
+
+  var peer  := new Object.make(protoTypesX, {prev}, os, "p"+natToString(i), pbound);
+  prev := spine;
+
+  os := os + {spine, peer};
+  oq := oq + [spine, peer];
+}
+
+print "Ownership - Directly Inside =========================\n\n";
+
+      for i := 0 to |oq|
+       {
+        print oq[i].nick;
+//         printobj(oq[i]);
+         print " owns ";
+
+         for j := 0 to |oq|
+{
+         print (if (directlyInside(oq[j],oq[i])) then (oq[j].nick+" ") else "");
+}
+         print "\n";
+
+       }
+  print "\n\n";
+
+
+print "Owners & Bound =========================\n\n";
+
+      for i := 0 to |oq|
+       {
+        print oq[i].nick;
+//         printobj(oq[i]);
+
+         print " owner=";
+         for j := 0 to |oq|
+         {
+         print (if (directlyInside(oq[i],oq[j])) then (oq[j].nick+" ") else "");
+         }
+
+         print " bound=";
+         for j := 0 to |oq|
+         {
+         print (if (directlyBounded(oq[i],oq[j])) then (oq[j].nick+" ") else "");
+         }
+
+         print "\n";
+
+       }
+  print "\n\n";
+
+
+
+
+//
+//
+// print "Ownership - Directly Inside =========================\n\n";
+//
+//       for i := 0 to |oq|
+//        {
+//         print oq[i].nick;
+// //         printobj(oq[i]);
+//          print "  ";
+//
+//          for j := 0 to |oq|
+// {
+//          print (if (directlyInside(oq[i],oq[j])) then (oq[i].nick+"<<"+oq[j].nick) else "      ");
+//          print " ";
+// }
+//          print "\n";
+//
+//        }
+//   print "\n\n";
+
+
+print "Ownership - Inside =========================\n\n";
+
+//       for i := 0 to |oq|
+//        {
+//          printobj(oq[i]);
+//          print "  ";
+//
+//          for j := 0 to |oq|
+// {
+//          print (if (inside(oq[i],oq[j])) then "i" else " ");
+//          print " ";
+// }
+//          print "\n";
+//
+//        }
+//   print "\n\n";
+
+      for i := 0 to |oq|
+       {
+        print oq[i].nick;
+//         printobj(oq[i]);
+         print "  ";
+
+         for j := 0 to |oq|
+{
+         print (if (inside(oq[i],oq[j])) then (oq[i].nick+"<="+oq[j].nick) else "      ");
+         print " ";
+}
+         print "\n";
+
+       }
+  print "\n\n";
+
+
+
+print "\n\nREFERENCE OK refOK =========================\n";
+print "REFERENCE OK refOK =========================\n\n";
+
+      for i := 0 to |oq|
+       {
+         print oq[i].nick;
+         //printobj(oq[i]);
+         print "  ";
+
+         for j := 0 to |oq|
+{
+         print (if (refOK(oq[i],oq[j])) then (oq[i].nick+"->"+oq[j].nick) else "    ");
+         print " ";
+}
+print "\n";
+}
+
+
+
+
+  print "\n[\n";
+
+      for i := 0 to |oq|
+       {
+         print "\"";
+
+         for j := 0 to |oq|
+{
+         print (if (refOK(oq[i],oq[j])) then ("x") else " ");
+}
+         if (i < (|oq|-1))  { print "\",\n";} else { print "\"\n";}
+
+       }
+print "]\n";
+
+
+} //end Main4
